add traces, missing last one for good model

process.v
@@ -154,10 +154,86 @@ Definition loop_and_count
  very cool, this still wroks for bad example too because we will switch to disk handler after next output
  This is similar to cpu cycle where we check the ic at the end of the cycle.*)
 
+
+(*Example*)
+
 Definition mask := Bool.
 Definition pending := Bool.
 Definition I_bits := Times pending mask.
-Definition ic := Arrow TInterrupt I_bits.
+Definition ic := Times I_bits (Times I_bits I_bits). (*new definition*)
+Definition count := Nat.
+Definition re_sch := Bool.
+Definition prev_pid := Option Nat.
+Definition cur_pid := Nat.
+Definition pids := Times cur_pid prev_pid.
+Definition bool_state := Times re_sch ic.
+(* I_list removed: all interrupts are always present *)
+Definition all_interrupts : seq [TInterrupt] :=
+  [:: TimerInterrupt; DiskInterrupt; DefaultInterrupt].
+Definition stateType := Times pids bool_state.
+
+Definition get_pids (v : [stateType]) := v.1.
+Definition get_bool_state (v : [stateType]) := v.2.
+Definition get_cur_pid (v : [stateType]) := (get_pids v).1.
+Definition get_prev_pid (v : [stateType]) := (get_pids v).2.
+Definition get_re_sch (v : [stateType]) := (get_bool_state v).1.
+Definition get_ic (v : [stateType]) := (get_bool_state v).2.
+
+Definition get_I_bits' (ic : [ic]) (ir : [TInterrupt]) : [I_bits] :=
+  match ir with
+  | DefaultInterrupt   => ic.1
+  | DiskInterrupt    => ic.2.1
+  | TimerInterrupt => ic.2.2
+  end.
+Definition get_I_bits (v : [stateType]) (ir : [TInterrupt]) := get_I_bits' (get_ic v) ir.
+
+Definition get_pending' (bits : [I_bits]) := bits.1.
+Definition get_mask' (bits : [I_bits]) := bits.2.
+
+Definition get_I_pending (v : [stateType]) (ir : [TInterrupt]) := get_pending' (get_I_bits v ir).
+Definition get_I_mask (v : [stateType]) (ir : [TInterrupt]) := get_mask' (get_I_bits v ir).
+
+Definition update_pids (v : [stateType]) pids : [stateType] := (pids,v.2).
+Definition update_bool_state (v : [stateType]) bs : [stateType] := (v.1,bs).
+Definition update_cur_pid (v : [stateType]) cur_pid : [stateType] := update_pids v (cur_pid,(get_pids v).2).
+Definition update_prev_pid (v : [stateType]) prev_pid : [stateType] := update_pids v ((get_pids v).1,prev_pid).
+Definition update_re_sch (v : [stateType]) re_sch : [stateType] := update_bool_state v (re_sch,(get_bool_state v).2).
+
+Definition update_I_bits' (myic : [ic]) (ir : [TInterrupt]) (bits : [I_bits]) : [ic] :=
+  match ir with
+  | DefaultInterrupt  => (bits, myic.2)
+  | DiskInterrupt    => (myic.1, (bits, myic.2.2))
+  | TimerInterrupt => (myic.1, (myic.2.1, bits))
+  end.
+
+Definition update_ic (v : [stateType]) ic : [stateType] := update_bool_state v ((get_bool_state v).1,ic).
+Definition update_I_bits (v : [stateType]) (ir : [TInterrupt]) (bits : [I_bits]) := update_ic v (update_I_bits' (get_ic v) ir bits).
+
+Definition update_I_pending (v : [stateType]) (ir : [TInterrupt]) pending : [stateType] :=
+  update_I_bits v ir (pending,get_I_mask v ir).
+Definition update_I_mask (v : [stateType]) (ir : [TInterrupt ]) mask : [stateType] :=
+  update_I_bits v ir (get_I_pending v ir,mask).
+
+Definition or_I_bits (b1 b2 : [I_bits]) : [I_bits] := (b1.1 || b2.1, b1.2 || b2.2).
+Definition or_ic (c1 c2 : [ic]) : [ic] :=
+  (or_I_bits c1.1 c2.1,
+   (or_I_bits c1.2.1 c2.2.1,
+    or_I_bits c1.2.2 c2.2.2)).
+Definition or_bool_state (s1 s2 : [bool_state]) : [bool_state] := (s1.1 || s2.1, or_ic s1.2 s2.2).
+
+Definition set_masks (v : [stateType]) : [stateType] :=
+  foldr (fun I v' => update_I_mask v' I true) v all_interrupts.
+Definition unset_masks (v : [stateType]) : [stateType] :=
+  foldr (fun I v' => update_I_mask v' I false) v all_interrupts.
+Definition masks_set (v : [stateType]) :=
+  foldr (fun I b => (get_I_mask v I) && b) true all_interrupts.
+
+
+(*Definition mask := Bool.
+Definition pending := Bool.
+Definition I_bits := Times pending mask.
+(*Definition ic := Arrow TInterrupt I_bits.*)
+Definition ic := Times I_bits (Times I_bits I_bits).
 Definition count := Nat.
 Definition re_sch := Bool.
 Definition prev_pid := Option Nat.
@@ -167,14 +243,6 @@ Definition pids := Times cur_pid prev_pid.
 Definition bool_state := Times re_sch ic.
 Definition I_list := List TInterrupt.
 Definition stateType := Times pids (Times I_list bool_state).
-
-(*Example*)
-Definition my_f_I (n : nat) := fun (n' : nat) => if n' == n.+2 then THandlerOutput else Unit.
-
-Definition I_output_type := Times THandlerOutput bool_state.
-
-Definition my_f_O (n : nat) := fun (n' : nat) => if n' == n.+1 then Nat (*handler*) else if n' == n.+2 then TTypeSyscall else if n' == n.+3 then TPublicOutput else I_output_type.
-
 
 (*Definition get_count (v : [stateType]) := v.1.1.*)
 Definition get_pids (v : [stateType]) := v.1.
@@ -217,13 +285,22 @@ Definition or_bool_state (s1 s2 : [bool_state]) : [bool_state] := (s1.1 || s2.1,
 Definition set_masks (v : [stateType]) : [stateType] := foldr (fun I v' => update_I_mask v' I true) v (get_I_list v).
 Definition unset_masks (v : [stateType]) : [stateType] := foldr (fun I v' => if I \in get_I_list v then update_I_mask v' I false else v') v (get_I_list v).
 Definition masks_set (v : [stateType]) := foldr (fun I b => (get_I_mask v I) && b) true (get_I_list v).
+*)
+
+
+Definition my_f_I := fun (n : nat) => if n == 4 then THandlerOutput else Unit.
+
+Definition I_output_type := Times THandlerOutput bool_state.
+
+Definition my_f_O := fun (n : nat) => if n == 3 then Nat else if n == 4 then TTypeSyscall else if n == 5 then TPublicOutput else I_output_type.
+
 
 Definition T_in := Sum TInterrupt Unit.
-Definition T_out' (handler_count : nat) := Times (Option TPublicOutput) (Times (Option TTypeSyscall) (Times (Option Nat) (times_on handler_count (fun _ => I_output_type)))).
+Definition T_out' := Times (Option TPublicOutput) (Times (Option TTypeSyscall) (Times (Option Nat) (times_on 2 (fun _ => I_output_type)))).
 Definition T' := Option THandlerOutput.
-Definition is_sch_out (n : nat) (o : [T_out' n]) :=
+Definition is_sch_out (o : [T_out']) :=
   match o with
-  | (None,(None,(Some n',_))) => Some n'
+  | (None,(None,(Some n,_))) => Some n
   | _ => None                                   
   end.
 
@@ -234,50 +311,45 @@ Definition is_I_in (i : [T_in]) :=
   end.
 
 (*Definition all_interrupts : seq [TInterrupt] := [::TimerInterrupt;DiskInterrupt].*)
-Definition n_to_I (v : [stateType]) (n : nat) := nth TimerInterrupt (get_I_list v) n.
+Definition n_to_I (v : [stateType]) (n : nat) := nth TimerInterrupt all_interrupts n.
 
-(* generic version of
-match i with
-  | (_,(Some (Notify,bstate),_)) => Some (TimerInterrupt,bstate)
-  | (Some (Notify,bstate),_) => Some (DiskInterrupt,bstate)
-  | _ => None
-  end.*)
-Definition is_I_out_done (v : [stateType]) (n : nat) (i : [T_out' n]) : [Option (Times TInterrupt bool_state)].
-  case: i. move=>_.
-  case. move=>_. 
-  case. move=>_.
-  elim: n. simpl. case. case. move=>_. intros. apply Some. exact (n_to_I v 0,b). exact None.
-  simpl. intros.
-  case: b. case. case. move=>_. intros. apply Some. exact (n_to_I v n.+1, b).
-  intros. apply H in b. apply b.
-Defined.    
+Definition tI_out (o : [T_out']) :=
+  match o with
+  | (_,(_,(_,(_,(_,x))))) => x
+  end.
 
+Definition dI_out (o : [T_out']) :=
+  match o with
+  | (_,(_,(_,(_,(x,_))))) => x
+  end.
 
-(*Definition is_I_out_running (i : [T_out']) :=
-  match i with
-  | (_,(Some (Nothing,_),_)) => Some TimerInterrupt
-  | (Some (Nothing,_),_) => Some DiskInterrupt
-  | _ => None
-  end.*)
+Definition default_I_out (o : [T_out']) :=
+  match o with
+  | (_,(_,(_,(x,(_,_))))) => x
+  end.  
+
+Definition is_I_out_done (o : [T_out']) : [Option (Times TInterrupt bool_state)] :=
+  if tI_out o is Some (Notify,b) then Some (TimerInterrupt,b)
+  else if dI_out o is Some (Notify,b) then Some (DiskInterrupt,b)
+  else if default_I_out o is Some (Notify,b) then Some (DefaultInterrupt,b)
+  else None.          
 
 
-
-Definition is_user_pid (p : [cur_pid]) : bool := (p < 2).
-Definition is_handler_pid (p : [cur_pid]) : bool := (2 < p).
+Definition is_user_pid (p : [cur_pid]) : bool := (3 < p).
+Definition is_sch (p : [cur_pid]) : bool := p == 3.
+Definition handler_pid := 3.
+Definition is_handler_pid (p : [cur_pid]) : bool := p == handler_pid.
 
 (* interrupt handlers live at pids 3 (timer) and 4 (disk) *)
-Definition I_handler_pid (v : [stateType]) (ir : [TInterrupt]) : [cur_pid] :=
-  3 + index TimerInterrupt (get_I_list v).
+Definition I_handler_pid (ir : [TInterrupt]) : [cur_pid] :=
+  index ir all_interrupts.
 
 (* a handler is selectable iff pending and not masked *)
 Definition I_ready (v : [stateType]) (ir : [TInterrupt]) : bool :=
   get_I_pending v ir && ~~ get_I_mask v ir.
 
-(*in prioritised order*) Locate all_interrupts.
-
-
 Definition first_ready (v : [stateType]) : option [TInterrupt] :=
-  ohead [seq ir <-  get_I_list v | (I_ready v ir) ].
+  ohead [seq ir <-  all_interrupts | (I_ready v ir) ].
 
 (* before overriding cur_pid, save it to prev_pid if it is a user process *)
 Definition save_cur_to_prev (v : [stateType]) : [stateType] :=
@@ -296,41 +368,40 @@ output scenarios
  *)
 
 (*issues*)
-Definition f_I (n : nat) (i : [Sum T_in (T_out' n)]) (v : [stateType]) : [stateType] :=
+Definition f_I (i : [Sum T_in T_out']) (v : [stateType]) : [stateType] :=
   match i with
   | inl i => if is_I_in i is Some ir then update_I_pending v ir true else v
-  | inr o => let v' := if @is_sch_out n o is Some n then update_cur_pid v n else v in (*apply scheduler choice, lowest priority*)
-             let v'':= if is_I_out_done v o is Some (ir,bstate) then
-                         update_bool_state v' (or_bool_state (get_bool_state (unset_masks v')) bstate) else v in
-             match first_ready v'' with
-             | Some ir => (update_I_pending (set_masks (update_cur_pid (save_cur_to_prev v) (I_handler_pid v ir))) ir false)
-             | None => if is_I_out_done v o is None then v
+  | inr o => let v := if @is_sch_out o is Some n then update_cur_pid v n else v in (*apply scheduler choice, lowest priority*)
+             let v:= if is_I_out_done o is Some (ir,bstate) then
+                         update_bool_state v (or_bool_state (get_bool_state (unset_masks v)) bstate) else v in
+             match first_ready v with
+             | Some ir => (update_I_pending (set_masks (update_cur_pid (save_cur_to_prev v) (I_handler_pid ir))) ir false)
+             | None => if is_I_out_done o is None then v
                        else if (get_re_sch v)
-                            then update_re_sch (update_prev_pid (update_cur_pid v 2) None) false
-                            else update_prev_pid (update_cur_pid v (odflt 2 (get_prev_pid v))) None
+                            then update_re_sch (update_prev_pid (update_cur_pid v handler_pid) None) false
+                            else update_prev_pid (update_cur_pid v (odflt handler_pid (get_prev_pid v))) None
              end
   end.
 
+(*We only reroute disk interrupts*)
+Definition is_I_out (o : [T_out']) : [Option THandlerOutput] :=
+  if dI_out o is Some (o',_) then Some o' else None.
+(*  
+  if tI_out o is Some (o',_) then Some o'
+  else if dI_out o is Some (o',_) then Some o'
+  else if default_I_out o is Some (o',b) then Some o'
+       else None.
+*)
 
-Definition is_I_out (n : nat) (i : [T_out' n]) : [Option THandlerOutput].
-  case: i. move=>_.
-  case. move=>_. 
-  case. move=>_.
-  elim: n. simpl. case. case. intros. exact (Some a). exact None.
-  simpl. intros.
-  case: b. case. case. intros. exact (Some a).
-  intros. apply H in b. apply b.
-Defined.
-
-Definition f_si (n : nat) (si : [Times stateType (Sum T_in (T_out' n))]) : [Option (Times Nat T')] :=
-  if si.2 is inr o then Some (get_cur_pid si.1, @is_I_out n o) else None.
+Definition f_si (si : [Times stateType (Sum T_in T_out')]) : [Option (Times Nat T')] :=
+  if si.2 is inr o then Some (get_cur_pid si.1, @is_I_out o) else None.
 
 Definition low_p := @out Unit TPublicOutput GetRequest.
 Definition high_p := @alternate_generic2 THandlerOutput TTypeSyscall Unit1 Syscall NOP tt (fun i => i == Notify).
 
 Definition handler_type := Proc Unit I_output_type.
-Definition false_ic : [ic] := fun _ => (false,false).
-
+Definition false_I_bits : [I_bits] := (false,false).
+Definition false_ic : [ic] := (false_I_bits,(false_I_bits,false_I_bits)).
 
 Definition I_handler (b: [bool_state]) : handler_type.
   rewrite /handler_type.
@@ -342,106 +413,194 @@ Definition I_handler (b: [bool_state]) : handler_type.
   apply out. exact tt.
 Defined.
 
-
 Definition bad_tI_handler : handler_type := I_handler (true,false_ic).
 Definition bad_dI_handler : handler_type := I_handler (false,false_ic).
 Definition bad_default_handler : handler_type := I_handler (false,false_ic).
 
-
-  
 Definition scheduler : Proc Unit Nat.
   eapply map. exact id.
-  instantiate (1:= Times Nat Unit). exact fst.
+  instantiate (1:= Times Nat Unit). exact (fun o => fst o + 4). (*skip first three processes to reach high_p (0) and low_p (1) *)
   eapply sta. exact (fun _ v => v). exact (fun _ v => v.+1%%2).
-  exact 0.
+  exact 1. (*Will start scheduling high process*)
   apply out. exact tt.
 Defined.
 
-Definition my_procs_bad : forall n, Proc (@my_f_I 1 n) (my_f_O 1 n).
+Definition my_procs_bad : forall n, Proc (my_f_I n) (my_f_O n).
   case. apply bad_tI_handler.
   case. apply bad_dI_handler.
-  case. apply scheduler.
+  case. apply bad_default_handler.
+  case. cbv. apply scheduler.
   case. apply high_p.  
   case. apply low_p.
   elim. apply bad_default_handler.
   intros. apply bad_default_handler.
 Defined.
-Definition my_f_coopt (n : nat) : bool := true.
-Definition my_f_initial (n : nat) := n == 0. 
-Definition f_proj (n : nat) (i : [T']) : forall n', [Option (my_f_I n n')].
+
+Print T'.
+
+Definition f_proj (i : [T']) : forall n, [Option (my_f_I n)].
   simpl. rewrite /my_f_I. intros. case_if.
   apply i.
-  exact (Some tt).
+  exact None. 
 Defined.
-Definition my_procs : forall n, Proc (@my_f_I 1 n) (my_f_O 1 n).
-  case. apply bad_tI_handler.
-  case. apply bad_dI_handler.
-  case. apply scheduler.
-  case. apply high_p.  
-  case. apply low_p.
-  elim. apply bad_default_handler.
-  intros. apply bad_default_handler.
-Defined.
-Definition my_process_pool_bad := @process_pool 4 my_f_coopt my_f_initial (my_f_I 1) (my_f_O 1) T' (f_proj 1) my_procs.
-Definition initial_state_bad : [stateType] := ((0,None),([::TimerInterrupt;DiskInterrupt],(false,(fun _ => (false,false))))).
-Definition def : [ (T_out' 1) ]  := (None,(None,(None,(None,None)))).
-Definition model_bad := @loop_and_count stateType initial_state_bad T_in (T_out' 1) T' (@f_I 1) def my_process_pool_bad (@f_si 1).
+
+Definition my_f_coopt (n : nat) : bool := true.
+Definition initial_pid := 5. (*starting with low process*)
+Definition my_f_initial (n : nat) := n == initial_pid.
+Definition my_process_pool_bad := @process_pool 5 my_f_coopt my_f_initial my_f_I my_f_O T' f_proj my_procs_bad.
+Definition initial_state_bad : [stateType] := ((initial_pid,None),(false,false_ic)).
+Definition def : [ T_out' ]  := (None,(None,(None,(None,(None,None))))).
+
+Definition model_bad : Proc T_in T_out' := @loop_and_count stateType initial_state_bad T_in T_out' T' f_I def my_process_pool_bad f_si.
+
+Definition Tsum' := ([T_in] + [T_out'])%type.
+
+Definition inr_tt : Tsum' := inl (inr tt).
+Definition dI' : Tsum' := inl (inl DiskInterrupt).
+Definition tI' : Tsum' := inl (inl TimerInterrupt). 
+Definition low_out x : [T_out'] := (Some x,(None,(None,(None,(None,None))))).
+Definition high_out x : [T_out'] := (None,(Some x,(None,(None,(None,None))))).
+Definition sch_o x : [T_out'] := (None,(None,(Some x,(None,(None,None))))).
+Definition defaultI_o x : [T_out'] := (None,(None,(None,(Some x,(None,None))))).
+Definition dI_o x : [T_out'] := (None,(None,(None,(None,(Some x,None))))).
+Definition tI_o x : [T_out'] := (None,(None,(None,(None,(None,Some x))))).
+
+Definition tI_yes' : Tsum' :=  inr (tI_o (Notify,(true,false_ic))).
+Definition tI_no' : Tsum' :=  inr (tI_o (Nothing,(false,false_ic))).
+
+Definition dI_yes' : Tsum' :=  inr (dI_o (Notify,(false,false_ic))).
+Definition dI_no' : Tsum' :=  inr (dI_o (Nothing,(false,false_ic))).
+
+Definition pub_get' : Tsum' := inr (low_out GetRequest).
+Definition pr_nop' : Tsum' := inr (high_out NOP).
+Definition pr_sys' : Tsum' := inr (high_out Syscall).
+
+Definition sch_low : Tsum' := inr (sch_o 5).
+Definition sch_high : Tsum' := inr (sch_o 4).
+
+Definition seqtype' := seq Tsum'.
+Eval cbv in T_out'.
+(*traces for bad model*) 
+Definition no_dI' : seqtype' :=   [::pub_get';                                     tI';pub_get';tI_no';tI_yes';sch_high;pr_nop'(*nop*);tI';pr_nop';tI_no';tI_yes';sch_low;pub_get'].
+Definition with_dI' : seqtype' := [::pub_get';dI';pub_get';dI_no';dI_yes';pub_get';tI';pub_get';tI_no';tI_yes';sch_high;pr_sys'(*sys*);tI';pr_nop';tI_no';tI_yes';sch_low;pub_get'].
+(*Definition with_dI' : seqtype' := [::tI';tI_no';tI_yes';sch_low;pub_get';dI';dI_no';dI_yes';pub_get';tI';tI_no';tI_yes';sch_high;pr_sys'(*sys*);pr_nop';tI';tI_no';tI_yes';pub_get'].*)
+
+(*Definition output_rel' := eqpair (eqmaybe (publicRel TPublicOutput)) (eqpair (eqmaybe (semiprivateRel TTypeSyscall)) (eqmaybe (semiprivateRel THandlerOutput))).*)
+(*Definition output_rel := eqmaybe (eqsum_R (publicRel TPublicOutput) (semiprivateRel TTypeSyscall)).*)
+
+Ltac rewr := rewrite /model_bad /loop_and_count /my_process_pool_bad /process_pool /my_f_initial /low_p /my_f_coopt /alternate_generic /alternate_generic2 /high_p /f_si /tI_o /bad_tI_handler /I_handler /f_proj /scheduler /bad_dI_handler /is_I_out /bad_default_handler /low_out.
+
+Ltac lsolv := try solve [ reduce_tac;reduce_tac | reduce_tac;try solve [reduce_once | econ];simpl;first (reduce_tac;reduce_tac)];simpl.
+Ltac reduce_tac2 :=
+  (try rewr);
+   (repeat
+      reduce_once);(try swi_instans); rewrite ?eqxx /= /xor /=.
+Lemma trace_no_dI' : forall l, Trace (publicRel _) l no_dI' model_bad.
+Proof.  
+  intros.
+  rewr;simpl;rewr;simpl;rewr;simpl;rewr.
+
+  do 12(first [econ;[idtac | econ | idtac] | econ];
+        reduce_tac;try solve [reflexivity| reduce_tac;reduce_tac];simpl;try swi_instans).
+
+  (*proved the last element of the trace manually to avoid evar holes in proof*)
+   (first [econ;[idtac | econ | idtac] | econ];
+    reduce_tac2;try solve [reflexivity| reduce_tac2;reduce_tac2];simpl;try swi_instans).
+   econ. reduce_tac2;reduce_tac2. econ. econ. reduce_tac. econ. econ.
+   reduce_tac. econ. econ. reduce_tac. econ. econ. reduce_tac. econ.
+   econ. reduce_tac. econ. econ. reduce_tac. econ.
+Qed.
+
+Lemma trace_with_dI' : forall l, Trace (publicRel _) l with_dI' model_bad.
+Proof.
+  intros.
+  rewr;simpl;rewr;simpl;rewr;simpl;rewr.
+
+  do 17(first [econ;[idtac | econ | idtac] | econ];
+        reduce_tac;try solve [reflexivity| reduce_tac;reduce_tac];simpl;try swi_instans).
+
+  (*proved the last element of the trace manually to avoid evar holes in proof*)  
+   (first [econ;[idtac | econ | idtac] | econ];
+    reduce_tac2;try solve [reflexivity| reduce_tac2;reduce_tac2];simpl;try swi_instans).
+   econ. reduce_tac2;reduce_tac2. econ. econ. reduce_tac. econ. econ.
+   reduce_tac. econ. econ. reduce_tac. econ. econ. reduce_tac. econ.
+   econ. reduce_tac. econ. econ. reduce_tac. econ.
+Qed.   
+
+Definition good_ic := ((false,true),((false,true),(false,false))).
+
+Definition initial_state_good : [stateType] := ((initial_pid,None),(false,good_ic)).
+
+Definition T'_good := Times (Option THandlerOutput) Bool.
+
+Definition to_T'_good (o : [T_out']) : [T'_good] :=
+  let b := if tI_out o is Some (Notify,_) then true else false in
+  let o' := if dI_out o is Some (o',_) then Some o' else None in
+  (o',b).
+
+Definition my_f_I_good := fun (n : nat) => if n == 0 then Unit else if n == 4 then THandlerOutput else if n < 3 then Bool else Unit.
 
 
-
-Definition initial_state_good : [stateType] := ((0,None),([::TimerInterrupt;DiskInterrupt;DefaultInterrupt],(false,(fun ir => if ir is TimerInterrupt then (false,false) else (false,true))))).
-
-Definition my_f_I_good (n : nat) := fun (n' : nat) => if n' == n.+1 then Unit else if n' == n.+2 then THandlerOutput else if n' == n.+3 then Unit else Bool.
-
-Definition T'_good := Option (Times THandlerOutput Bool).
-(*We extend the input to schedulers so we can distinguish if the latest output was from a timer interrupt.
+    
+(*We extend the input to schedulers so we can distinguish if the latest output was Notify by timer interrupt.
  This will feed their counter.
  true = from finishing timer interrupt, reset counter
  false = output pulse, decrement counter*)
-Definition f_proj_good (n : nat) (i : [T'_good]) : forall n', [Option (my_f_I_good n n')].
+Definition f_proj_good (i : [T'_good]) : forall n, [Option (my_f_I_good n)].
   simpl. rewrite /my_f_I_good. intros.
-  case_if. exact None.
-  case_if. destruct i. destruct i. exact (Some i). exact None.
-  case_if. exact None.
-  destruct i. destruct i. exact (Some i0). exact None.
+  case_if. exact None. (*timer interrupt handler does not need any information*)
+  case_if.
+  exact (fst i).
+  case_if. exact (Some (snd i)). (*other interrupts receive bool, true -> timer interrupt just finished, set count = 2, false -> decrement counter*)
+  exact None.
 Defined.  
 
 Definition good_handler_type := Proc Bool I_output_type.
-Definition default_on_ic : [ic] := fun (ir :[TInterrupt]) => if ir is DefaultInterrupt then (true,false) else (false,false).
-Definition mask_most : [ic] := fun (ir :[TInterrupt]) => if ir is TimerInterrupt then (false,false) else (false,true).
-Definition good_I_handler (b : [bool_state]) : good_handler_type.
+Definition default_on_ic : [ic] := ((true,false),((false,false),(false,false))). (*pending set for default*)
+Definition mask_most : [ic] := ((false,true),((false,true),(false,false))). (*mask set for everything but timer interrupt*)
+
+(*n = time slice*)
+(*We assume that when the running handler is stopped by the timer, it has finished its work.
+ Enforced by allowing time slice of 2.
+ The two units are consumed by disk interrupt or default interrupt, in that order, if either or both their pending bits are set.
+ If the timer interrupt runs again before either of the two other handlers then after completing the time slice will again be 2.
+ All handlers take 2 units of time to complete, so by enforcing a time slice equal to length of a handler we never stop handlers mid execution.
+ Assuming all handlers take the same amount of time and that we don't interrupt mid handling, are simplifying assumptions.
+ *)
+Definition good_I_handler (n : nat) (b : [bool_state]) : good_handler_type.
   eapply map. exact id.
   2: eapply sta.
   instantiate (2:= Nat).
   instantiate (1:= I_output_type).
-  exact (fun o => if o.1 != 0 then o.2 else (Notify,(false,mask_most))).
-  exact (fun b n => if b then 4 else n.-1).
-  exact (fun o n => n).
-  exact 4.
+  exact (fun o => if o.1 != 0 then o.2 else (o.2.1,or_bool_state o.2.2 (false,mask_most))). (*in the else case, o.2.1 will always be Notify and o.2.2 will be b*)
+  exact (fun b n' => if b then n else n').
+  exact (fun o n' => n'.-1).
+  exact n.
   eapply map. instantiate (1:= Unit). exact (fun i => tt). exact id.
   apply (I_handler b).
 Defined.
 
-Definition good_tI_handler : good_handler_type := good_I_handler (true,default_on_ic).
-Definition good_dI_handler : good_handler_type := good_I_handler (false,default_on_ic).
-Definition good_default_handler : good_handler_type := good_I_handler (false,default_on_ic).      
+Definition time_slice := 2. 
+Definition good_tI_handler : handler_type := I_handler (true,default_on_ic).
+Definition good_dI_handler : good_handler_type := good_I_handler time_slice (false,default_on_ic).
+Definition good_default_handler : good_handler_type := good_I_handler time_slice (false,default_on_ic).      
 
-Definition my_good_procs : forall n, Proc (@my_f_I_good 2 n) (my_f_O 2 n).
+Definition my_good_procs : forall n, Proc (@my_f_I_good n) (my_f_O n).
   case. apply good_tI_handler.
   case. apply good_dI_handler.
   case. apply good_default_handler.
   case. apply scheduler.
   case. apply high_p.
   case. apply low_p.
-  elim. apply good_default_handler.
-  intros. apply good_default_handler.
+  elim. apply bad_default_handler.
+  intros. apply bad_default_handler.
 Defined.
 
-Definition my_process_pool_good := @process_pool 5 my_f_coopt my_f_initial (my_f_I_good 2) (my_f_O 2) T'_good  (@f_proj_good 2) my_good_procs.
+Definition my_process_pool_good := @process_pool 5 my_f_coopt my_f_initial my_f_I_good my_f_O T'_good f_proj_good my_good_procs.
 
-Definition def_good : [ (T_out' 2) ]  := (None,(None,(None,(None,(None,None))))).
+Definition def_good : [ T_out' ]  := (None,(None,(None,(None,(None,None))))).
 
-Definition is_I_out_good (i : [T_out' 2]) : [T'_good].
+(*Definition is_I_out_good (i : [T_out']) : [T'_good].
   case: i. move=>_.
   case. move=>_. 
   case. move=>_.
@@ -449,19 +608,135 @@ Definition is_I_out_good (i : [T_out' 2]) : [T'_good].
   case. case. case=>h. intros. exact (Some (h,false)).
   case. case. case=>h. intros. exact (Some (h,false)).
   case. case=>h. intros. exact (Some (h,true)). exact None.
-Defined.
+Defined.*)
 
-Definition f_si_good (si : [Times stateType (Sum T_in (T_out' 2))]) : [Option (Times Nat T'_good)] :=
-  if si.2 is inr o then Some (get_cur_pid si.1, is_I_out_good o) else None.
+Definition f_si_good (si : [Times stateType (Sum T_in T_out')]) : [Option (Times Nat T'_good)] :=
+  if si.2 is inr o then Some (get_cur_pid si.1, to_T'_good o) else None.
 
-Definition model_good := @loop_and_count stateType initial_state_good T_in (T_out' 2) T'_good (@f_I 2) def_good my_process_pool_good f_si_good.
-
-
-
-
+Definition model_good := @loop_and_count stateType initial_state_good T_in T_out' T'_good f_I def_good my_process_pool_good f_si_good.
+Print model_bad.
+Print model_good.
 
 
+Definition tI_no'g : Tsum' :=  inr (tI_o (Nothing,(false,false_ic))).
+Definition tI_yes'g : Tsum' :=  inr (tI_o (Notify,(true,default_on_ic))).
 
+Definition default_and_masked_ic := or_bool_state (false, default_on_ic) (false, mask_most).
+                                     
+Definition defaultI_no'g : Tsum' :=  inr (defaultI_o (Nothing,(false,false_ic))).
+Definition defaultI_yes'g : Tsum' :=  inr (defaultI_o (Notify,default_and_masked_ic)).
+
+
+Definition good_no_dI' : seqtype' :=   [::pub_get';                        tI';pub_get';tI_no'g;tI_yes'g;defaultI_no'g;defaultI_yes'g;sch_high;pr_nop'(*nop*);tI';pr_nop';tI_no'g;tI_yes'g;defaultI_no'g;defaultI_yes'g;sch_low;pub_get'].
+Definition good_with_dI' : seqtype' :=   [::pub_get';dI';pub_get';pub_get';tI';pub_get';tI_no'g;tI_yes'g;defaultI_no'g;defaultI_yes'g;sch_high;pr_sys'(*sys*);tI';pr_nop';tI_no'g;tI_yes'g;defaultI_no'g;defaultI_yes'g;sch_low;pub_get'].
+
+
+Ltac rewr ::= rewrite /model_bad /loop_and_count /my_process_pool_bad /process_pool /my_f_initial /low_p /my_f_coopt /alternate_generic /alternate_generic2 /high_p /f_si /tI_o /bad_tI_handler /I_handler /f_proj /scheduler /bad_dI_handler /is_I_out /bad_default_handler /low_out /model_good /my_process_pool_good /f_si_good /to_T'_good /f_proj_good /good_default_handler /good_tI_handler /good_dI_handler /good_I_handler.
+
+
+
+Lemma trace_good_no_dI' : forall l, Trace (publicRel _) l good_no_dI' model_good.
+Proof.  
+  intros.
+  rewr;simpl;rewr;simpl;rewr;simpl;rewr.
+
+  do 16(first [econ;[idtac | econ | idtac] | econ];
+        reduce_tac;try solve [reflexivity| reduce_tac;reduce_tac];simpl;try swi_instans).
+
+   (first [econ;[idtac | econ | idtac] | econ];
+    reduce_tac2;try solve [reflexivity| reduce_tac2;reduce_tac2];simpl;try swi_instans).
+   econ. reduce_tac2;reduce_tac2. econ. econ. reduce_tac. econ. econ.
+   reduce_tac. econ. econ. reduce_tac. econ. econ. reduce_tac. econ.
+   econ. reduce_tac. econ. econ. reduce_tac. econ.
+Qed.
+
+Lemma trace_good_with_dI' : forall l, Trace (publicRel _) l good_with_dI' model_good.
+Proof.  
+  intros.
+  rewr;simpl;rewr;simpl;rewr;simpl;rewr.
+
+  do 9(first [econ;[idtac | econ | idtac] | econ];
+        reduce_tac;try solve [reflexivity| reduce_tac;reduce_tac];simpl;try swi_instans).
+
+   (first [econ;[idtac | econ | idtac] | econ];
+    reduce_tac2;try solve [reflexivity| reduce_tac2;reduce_tac2];simpl;try swi_instans).
+   econ. reduce_tac2;reduce_tac2. econ. econ. reduce_tac. econ. econ.
+   reduce_tac. econ. econ. reduce_tac. econ. econ. reduce_tac. econ.
+   econ. reduce_tac. econ. econ. reduce_tac. econ.
+Qed.  
+
+ do 6(first [econ;[idtac | econ | idtac] | econ];
+       reduce_tac;try solve [reflexivity| reduce_tac;reduce_tac];simpl;try swi_instans).  
+
+  Eval cbv in ( (update_re_sch
+                   (update_prev_pid
+                      (update_cur_pid
+                         (update_bool_state
+                            (update_I_pending
+                               (set_masks
+                                  (update_cur_pid
+                                     (save_cur_to_prev
+                                        (update_I_pending initial_state_good TimerInterrupt true))
+                                     (I_handler_pid TimerInterrupt)))
+                               TimerInterrupt false)
+                            (or_bool_state
+                               (false,
+                                (get_I_pending
+                                   (update_I_pending
+                                      (set_masks
+                                         (update_cur_pid
+                                            (save_cur_to_prev
+                                               (update_I_pending initial_state_good TimerInterrupt
+                                                  true))
+                                            (I_handler_pid TimerInterrupt)))
+                                      TimerInterrupt false)
+                                   DefaultInterrupt,
+                                 false,
+                                 (get_I_pending
+                                    (update_I_mask
+                                       (update_I_pending
+                                          (set_masks
+                                             (update_cur_pid
+                                                (save_cur_to_prev
+                                                   (update_I_pending initial_state_good TimerInterrupt
+                                                      true))
+                                                (I_handler_pid TimerInterrupt)))
+                                          TimerInterrupt false)
+                                       DefaultInterrupt false)
+                                    DiskInterrupt,
+                                  false,
+                                  (get_I_pending
+                                     (update_I_mask
+                                        (update_I_mask
+                                           (update_I_pending
+                                              (set_masks
+                                                 (update_cur_pid
+                                                    (save_cur_to_prev
+                                                       (update_I_pending initial_state_good
+                                                          TimerInterrupt true))
+                                                    (I_handler_pid TimerInterrupt)))
+                                              TimerInterrupt false)
+                                           DefaultInterrupt false)
+                                        DiskInterrupt false)
+                                     TimerInterrupt,
+                                   false))))
+                               (true, default_on_ic)))
+                         handler_pid)
+                      None)
+                   false)).
+
+  econ. 2:econ. reduce_tac;reduce_tac.
+
+  Eval cbv in (update_I_pending initial_state_good TimerInterrupt true).
+
+  (*proved the last element of the trace manually to avoid evar holes in proof*)
+   (first [econ;[idtac | econ | idtac] | econ];
+    reduce_tac2;try solve [reflexivity| reduce_tac2;reduce_tac2];simpl;try swi_instans).
+   econ. reduce_tac2;reduce_tac2. econ. econ. reduce_tac. econ. econ.
+   reduce_tac. econ. econ. reduce_tac. econ. econ. reduce_tac. econ.
+   econ. reduce_tac. econ. econ. reduce_tac. econ.
+Qed.
+Lemma trace_good_with_dI' : forall l, Trace (publicRel _) l good_with_dI' model_good.
 
 
 
@@ -716,8 +991,7 @@ Definition handl_out : Tsum := inr None.
 Definition non' : Tsum' := inr (None,(None,None)).
 Definition non : Tsum := inr None.
 
-Definition no_dI' : seqtype' :=   [::handl_out_noth';pub_get';    pub_get';tI';handl_out_noth';pr_nop'(*nop*);pr_nop';tI';handl_out_noth';pub_get'].
-Definition with_dI' : seqtype' := [::handl_out_noth';pub_get';dI';pub_get';tI';handl_out_noti';pr_sys'(*sys*);pr_nop';tI';handl_out_noth';pub_get'].
+
 Definition no_dI : seqtype :=   [::handl_out;pub_get;    pub_get;tI;handl_out;pr_nop(*nop*);pr_nop;tI;handl_out;pub_get].
 Definition with_dI : seqtype := [::handl_out;pub_get;dI;pub_get;tI;handl_out;pr_sys(*sys*);pr_nop;tI;handl_out;pub_get].
 
@@ -756,10 +1030,7 @@ Lemma trace_with_dI' : forall l, Trace output_rel' l with_dI' model'.
 Qed.
 
 (*Necessary to avoid controlled_eauto tactic weirdness in reduce_tac*)
-Ltac reduce_tac2 :=
-  (try rewr);
-   (repeat
-      reduce_once);(try swi_instans); rewrite ?eqxx /= /xor /=.
+
 
 
 Lemma trace_no_dI : forall l, Trace output_rel l no_dI model.
@@ -829,8 +1100,6 @@ Lemma trace_with_dI : forall l, Trace output_rel l with_dI model.
 Qed.
 
 
-Definition bad_no_dI' : seqtype' :=   [::handl_out_noth';tI';pub_get';                                        pub_get';tI';pr_nop';pr_nop';tI';pub_get'].
-Definition bad_with_dI' : seqtype' := [::handl_out_noth';tI';pub_get';dI';handl_out_noti';pr_sys';pr_nop';tI';pub_get';tI';pr_nop';pr_nop';tI';pub_get'].
 
 Definition bad_no_dI : seqtype :=     [::handl_out;      tI; pub_get;                                         pub_get;tI;pr_nop;pr_nop;tI;pub_get].
 Definition bad_with_dI : seqtype :=   [::handl_out;tI;pub_get;dI;handl_out;pr_sys;pr_nop;tI;pub_get;tI;pr_nop;pr_nop;tI;pub_get].
